Rules.thy
@@ -24,8 +24,10 @@ inductive rules :: "'b rpred \<Rightarrow> 'b rpred \<Rightarrow> 'b set \<Right
   choice[intro]: "R,G \<turnstile> P { c\<^sub>1 } Q \<Longrightarrow> R,G \<turnstile> P { c\<^sub>2 } Q \<Longrightarrow> R,G \<turnstile> P { c\<^sub>1 \<sqinter> c\<^sub>2 } Q" |
   seqset[intro]: "\<forall>s \<in> S. R,G \<turnstile> P { seq2com s } Q \<Longrightarrow> R,G \<turnstile> P { \<Sqinter> S } Q" |
   loop[intro]:   "stable R P \<Longrightarrow> R,G \<turnstile> P { c } P \<Longrightarrow> R,G \<turnstile> P { c* } P" |
+  state[intro]:  "R,G \<turnstile> P { c } Q \<Longrightarrow> inter R G c \<Longrightarrow> 
+                  thr\<^sub>R op R,thr\<^sub>G op G \<turnstile> thr\<^sub>P op l P { State l op c } thr\<^sub>Q op Q" |
   thread[intro]: "R,G \<turnstile> P { c } Q \<Longrightarrow> inter R G c \<Longrightarrow> 
-                  thr\<^sub>R op R,thr\<^sub>G op G \<turnstile> thr\<^sub>P op l P { Thread l op c } thr\<^sub>Q op Q" |
+                  thr\<^sub>R op R,thr\<^sub>G op G \<turnstile> thr\<^sub>A op P { Thread op c } thr\<^sub>Q op Q" |
   par[intro]:    "R\<^sub>1,G\<^sub>1 \<turnstile> P\<^sub>1 { c\<^sub>1 } Q\<^sub>1 \<Longrightarrow> R\<^sub>2,G\<^sub>2 \<turnstile> P\<^sub>2 { c\<^sub>2 } Q\<^sub>2 \<Longrightarrow> G\<^sub>2 \<subseteq> R\<^sub>1 \<Longrightarrow> G\<^sub>1 \<subseteq> R\<^sub>2 \<Longrightarrow> 
                   R\<^sub>1 \<inter> R\<^sub>2,G\<^sub>1 \<union> G\<^sub>2 \<turnstile> P\<^sub>1 \<inter> P\<^sub>2 { c\<^sub>1 || c\<^sub>2 } (Q\<^sub>1 \<inter> Q\<^sub>2)" |
   conseq[intro]: "R,G \<turnstile> P { c } Q \<Longrightarrow> P' \<subseteq> P \<Longrightarrow> R' \<subseteq> R \<Longrightarrow> G \<subseteq> G' \<Longrightarrow> Q \<subseteq> Q' \<Longrightarrow> 
@@ -100,8 +102,11 @@ lemma stable_preE:
   shows "\<exists>P'. P \<subseteq> P' \<and> stable R P' \<and> R,G \<turnstile> P' {c} Q"
   using assms 
 proof (induct)
-  case (thread R G P c Q op l)
-  then show ?case by (metis thr_stable thr_mono rules.thread)
+  case (state R G P c Q op l)
+  then show ?case by (metis thr_stable thr_mono rules.state)
+next 
+  case (thread R G P c Q op)
+  then show ?case by (metis thr_stable' thr_mono' rules.thread)
 next 
   case (par R\<^sub>1 G\<^sub>1 P\<^sub>1 c\<^sub>1 Q\<^sub>1 R\<^sub>2 G\<^sub>2 P\<^sub>2 c\<^sub>2 Q\<^sub>2)
   obtain P\<^sub>1' where 1: "P\<^sub>1 \<subseteq> P\<^sub>1'" "stable R\<^sub>1 P\<^sub>1'" "R\<^sub>1,G\<^sub>1 \<turnstile> P\<^sub>1' {c\<^sub>1} Q\<^sub>1" using par by auto
@@ -138,10 +143,19 @@ next
   thus ?case using aux\<^sub>P_mono aux_stable by (metis rules.aux)
 qed blast+
 
-text \<open>A variant of the thread rule that eliminates all references to the local state\<close>
-lemma thread_allI:
-  "R,G \<turnstile> P { c } Q \<Longrightarrow> inter R G c \<Longrightarrow> thr\<^sub>R op R,thr\<^sub>G op G \<turnstile> thr\<^sub>A op P { Thread l op c } thr\<^sub>Q op Q"
-  by (rule conseq[OF thread]) (auto simp: thr\<^sub>A_def thr\<^sub>P_def)
+lemma false_seqI [intro]:
+  "\<forall>\<beta> \<in> set s. guar\<^sub>\<alpha> \<beta> G \<Longrightarrow> R,G \<turnstile> {} {seq2com s} {}"
+  by (induct s) auto
+
+lemma falseI:
+  shows "local c \<Longrightarrow> \<forall>\<beta> \<in> basics c. guar\<^sub>\<alpha> \<beta> G \<Longrightarrow> UNIV,G \<turnstile> {} { c } {}"
+proof (induct c)
+  case (Basic x)
+  thus ?case by (intro basic) (auto simp: atomic_rule_def guar_def wp_def)
+next
+  case (SeqChoice x)
+  thus ?case by (intro ballI seqset false_seqI) auto
+qed auto
 
 end
 
